Handle integers, comparison, conversion to BigInt
Implement BigInt axioms with Coq Z
Implement Int axioms with custom bounded int type (for now)
Add comparison functions in ident, ty
Replace gmap with Zmap
Add (OCaml) functions to convert to/from Z (need to test)
A little refactoring
Everything compiles

extract/BigInt.ml
@@ -92,3 +92,7 @@ let hash = Z.hash
 (*For convenience*)
 let is_zero (x: t) : bool = eq x zero
 let pos (x: t) : bool = compare x zero > 0
+
+(*Added*)
+let of_Z (x: Z.t) : t = x
+let to_Z (x: t) : Z.t = x
