extract/Ty.mli
@@ -23,7 +23,7 @@ module Mtv : Extmap.S with type key = tvsymbol
 module Stv : Extset.S with type elt = tvsymbol
 (*module Htv : Exthtbl.S with type key = tvsymbol*)
 
-(*val tv_compare : tvsymbol -> tvsymbol -> int*)
+val tv_compare : tvsymbol -> tvsymbol -> int
 val tv_equal : tvsymbol -> tvsymbol -> bool
 val tv_hash : tvsymbol -> BigInt.t
 
@@ -76,8 +76,8 @@ module Sty : Extset.S (*with module M = Mty
 module Hty : Exthtbl.S with type key = ty
 module Wty : Weakhtbl.S with type key = ty*)
 
-(*val ts_compare : tysymbol -> tysymbol -> int*)
-(*val ty_compare : ty -> ty -> int*)
+val ts_compare : tysymbol -> tysymbol -> int
+val ty_compare : ty -> ty -> int
 
 val ts_equal : tysymbol -> tysymbol -> bool
 val ty_equal : ty -> ty -> bool
@@ -176,7 +176,7 @@ val is_ts_tuple_id : ident -> int option*)
 
 exception UnexpectedProp
 
-(*val oty_compare : ty option -> ty option -> int*)
+val oty_compare : ty option -> ty option -> int
 val oty_equal : ty option -> ty option -> bool
 val oty_hash  : ty option -> BigInt.t
 
