extract/ZCompat.ml
@@ -1,0 +1,48 @@
+(*Convert between Coq Z and OCaml Z.t (for Zmap data structure)*)
+
+(*Requires a positive Z.t*)
+let to_pos (z: Z.t) : BinNums.positive =
+  let rec build_pos (n: int) (base: BinNums.positive) : BinNums.positive =
+    if n < 0 then base
+    else 
+      let b = Z.testbit z n in
+      if b then build_pos (n-1) (Coq_xI base)
+      else build_pos (n-1) (Coq_xO base)
+  in build_pos (Z.numbits z - 1) Coq_xH  
+
+let to_Z (z: Z.t) : BinNums.coq_Z =
+  if Z.equal z Z.zero then Z0
+  else if Z.gt z Z.zero then Zpos (to_pos z)
+  else Zneg (to_pos (Z.neg z))
+
+let of_pos (p: BinNums.positive) : Z.t =
+  let rec of_pos_aux (p: BinNums.positive) (z: Z.t) : Z.t =
+    match p with
+    | Coq_xH -> z
+    | Coq_xO p' -> of_pos_aux p' (Z.shift_left z 1) (*2 * z*)
+    | Coq_xI p' -> of_pos_aux p' (Z.succ (Z.shift_left z 1))(*2 * z + 1*)
+  in
+  of_pos_aux p Z.one
+
+let of_Z (z: BinNums.coq_Z) : Z.t =
+  match z with
+  | Z0 -> Z.zero
+  | Zpos p -> of_pos p
+  | Zneg p -> Z.neg (of_pos p)
+
+let to_Z_big = fun x -> to_Z (BigInt.to_Z x)
+let of_Z_big = fun x -> BigInt.of_Z (of_Z x)
+
+
+
+  (*OCaml function to_pos - gives positive of (x+1) because
+  we allow 0 values
+  (*Go from [numbits x]-1 down to 0*)
+  let to_pos (x: Z.t) = 
+    let rec build_pos (n: int) (x: Z.t) (base: positive) : positive =
+      if n < 0 then base else
+      let b = Z.testbit x n in
+      if b then build_pos (n-1) (xI base)
+      else build_pos (n-1) (xO base)
+    in build_pos (Z.numbits x - 1) (Z.succ x) xH
+*)
