src/util/CoqInt.v
@@ -1,14 +1,14 @@
-(*A light axiomatization of OCaml ints. We really don't need
-  very much*)
-(*Here, we use bounded ints so that we can extract directly
-  to OCaml's int type*)
-Parameter int : Type.
-Parameter int_eqb : int -> int -> bool.
-(*Parameter Abs : int -> Z.*)
-Parameter int_eqb_eq: forall (i1 i2: int), i1 = i2 <-> int_eqb i1 i2 = true.
+(*A light axiomatization/implementation of OCaml's ints.
+  We implement using Coq bounded ints but extract to
+  OCaml int. See comment in CoqBigInt.t*)
+Require Import Integer.
+Definition int : Type := int63.
+Definition int_eqb : int -> int -> bool := int63_eqb.
+(*NOTE: this is an axiom for OCaml*)
+(*TODO: better way of identifying axioms*)
+Definition int_eqb_eq : forall (i1 i2: int), i1 = i2 <-> int_eqb i1 i2 = true :=
+  int63_eqb_eq.
 
-(*We need to create a list of length n*)
-Parameter list_init: forall {A: Type}, int -> (int -> A) -> list A.
-
-Require Import Coq.Strings.String.
-Parameter string_of_int: int -> string.
+Definition zero : int := int63_of_Z 0%Z eq_refl.
+Definition one : int := int63_of_Z 1%Z eq_refl.
+Definition neg_one : int := int63_of_Z (-1)%Z eq_refl.
