extract/Extract.v
@@ -33,6 +33,7 @@ Extract Inlined Constant CoqBigInt.eqb => "BigInt.eq".
 Extract Inlined Constant CoqBigInt.mul_int => "BigInt.mul_int".
 Extract Inlined Constant CoqBigInt.add => "BigInt.add".
 Extract Inlined Constant CoqBigInt.lt => "BigInt.lt".
+Extract Inlined Constant CoqBigInt.compare => "BigInt.compare".
 Extract Inlined Constant CoqBigInt.two => "(BigInt.of_int 2)".
 Extract Inlined Constant CoqBigInt.three => "(BigInt.of_int 3)".
 Extract Inlined Constant CoqBigInt.four => "(BigInt.of_int 4)".
@@ -44,11 +45,17 @@ Extract Inlined Constant CoqBigInt.nine => "(BigInt.of_int 9)".
 
 Extract Inlined Constant CoqInt.int => "Int.t".
 Extract Inlined Constant CoqInt.int_eqb => "Int.equal".
+Extract Inlined Constant CoqInt.zero => "Int.zero".
+Extract Inlined Constant CoqInt.one => "Int.one".
+Extract Inlined Constant CoqInt.neg_one => "Int.minus_one".
 Extract Inlined Constant Hashcons.int_65599 => "65599".
 
+Extract Inlined Constant CoqBigInt.to_Z => "ZCompat.to_Z_big".
+Extract Inlined Constant CoqBigInt.of_Z => "ZCompat.of_Z_big".
+
 (*TODO: this is BAD - figure out better*)
-Extract Inlined Constant length => "List.length".
-Extract Inlined Constant Coq.Arith.PeanoNat.Nat.eqb => "Int.equal".
+(*Extract Inlined Constant length => "List.length".
+Extract Inlined Constant Coq.Arith.PeanoNat.Nat.eqb => "Int.equal".*)
 
 (*Handle exception monad*)
 
