src/util/IntFuncs.v
@@ -1,0 +1,67 @@
+(*Functions that operate on [CoqBigInt.t]. They must
+  ONLY use definitions/lemmas from that file. They cannot
+  refer to the fact that the type is secretly Z underneath*)
+Require CoqBigInt.
+Require Import Coq.Lists.List.
+Require Export Coq.ZArith.BinInt.
+Require Import Lia.
+
+Local Open Scope Z_scope.
+
+
+Fixpoint int_length {A: Type} (l: list A) : CoqBigInt.t :=
+  match l with
+  | nil => CoqBigInt.zero
+  | _ :: t => CoqBigInt.succ (int_length t)
+  end.
+
+Lemma int_length_nonneg {A: Type} (l: list A) :
+  0 <= CoqBigInt.to_Z (int_length l).
+Proof.
+  induction l; simpl.
+  - rewrite CoqBigInt.zero_spec. lia.
+  - rewrite CoqBigInt.succ_spec. lia.
+Qed.
+
+Lemma int_length_spec {A: Type} (l: list A) : 
+  Z.to_nat (CoqBigInt.to_Z (int_length l)) = List.length l.
+Proof.
+  induction l; simpl.
+  - rewrite CoqBigInt.zero_spec. reflexivity.
+  - rewrite CoqBigInt.succ_spec.
+    rewrite Znat.Z2Nat.inj_succ.
+    + rewrite IHl; reflexivity.
+    + apply int_length_nonneg.
+Qed. 
+
+(*TODO: move*)
+Lemma Z2Nat_eqb_nat (z1 z2: Z):
+  0 <= z1 ->
+  0 <= z2 ->
+  Nat.eqb (Z.to_nat z1) (Z.to_nat z2) = Z.eqb z1 z2.
+Proof.
+  intros Hz1 Hz2.
+  destruct (Z.eqb_spec z1 z2); subst; simpl.
+  - apply PeanoNat.Nat.eqb_refl.
+  - destruct (PeanoNat.Nat.eqb_spec (Z.to_nat z1) (Z.to_nat z2));
+    auto.
+    apply Znat.Z2Nat.inj_iff in e; auto. contradiction.
+Qed.
+    
+(*A corollary*)
+Lemma int_length_eq {A: Type} (l1 l2: list A):
+  CoqBigInt.eqb (int_length l1) (int_length l2) =
+  Nat.eqb (length l1) (length l2).
+Proof.
+  rewrite CoqBigInt.eqb_spec.
+  rewrite <- Z2Nat_eqb_nat; try solve[apply int_length_nonneg].
+  rewrite !int_length_spec. reflexivity.
+Qed.
+
+Definition option_compare {A: Type} (cmp:  A -> A -> CoqInt.int) (o1 o2: option A) : CoqInt.int :=
+  match o1, o2 with
+  | Some v0, Some v1 => cmp v0 v1
+  | None, None => CoqInt.zero
+  | None, Some _ => CoqInt.neg_one
+  | Some _, None => CoqInt.one
+  end.
