src/util/Integer.v
@@ -1,0 +1,54 @@
+(*A (limited) formalization of machine-length integers*)
+(*We could use CompCert's integers, but that is a pretty large
+dependency. For now, we avoid*)
+(*The main difference is that we use a boolean predicate
+  for computation and proof irrelevance.
+  Additionally, we are not concerned we signed/unsigned 
+  representations.
+  Really, we just want a bound. We don't use ints for much
+  except comparisons in OCaml*)
+Require Export Coq.ZArith.BinInt.
+From Proofs Require Import core.Common.
+
+Local Open Scope Z_scope.
+
+Section BoundedInt.
+
+Variable bound : Z. (*For Ocaml: 2 ^ 62*)
+
+(*Use boolean *)
+Record int := mk_int { int_val : Z; 
+  int_bound: Z.leb (-bound) int_val && Z.ltb int_val bound}.
+
+Definition eqb (i1 i2: int) : bool :=
+  Z.eqb (int_val i1) (int_val i2).
+
+Lemma eqb_spec (i1 i2: int): reflect (i1 = i2) (eqb i1 i2).
+Proof.
+  unfold eqb.
+  destruct (Z.eqb_spec (int_val i1) (int_val i2));
+  [apply ReflectT | apply ReflectF].
+  - destruct i1 as [i1 b1]; destruct i2 as [i2 b2];
+    simpl in *; subst.
+    assert (b1 = b2) by apply bool_irrelevance;
+    subst; reflexivity.
+  - intro C; subst; contradiction.
+Qed.
+
+Lemma eqb_eq (i1 i2: int) : i1 = i2 <-> eqb i1 i2.
+Proof.
+  destruct (eqb_spec i1 i2); subst; split; auto;
+  discriminate.
+Qed.
+
+End BoundedInt.
+
+Definition ocaml_int_size := 2 ^ 62.
+
+Definition int63 := int ocaml_int_size.
+Definition int63_eqb := eqb ocaml_int_size.
+Lemma int63_eqb_eq (i1 i2: int63) : i1 = i2 <-> int63_eqb i1 i2.
+Proof. apply eqb_eq. Qed.
+
+Definition int63_of_Z (z: Z) (Hz: Z.leb (-ocaml_int_size) z && Z.ltb z ocaml_int_size) : int63 :=
+  mk_int _ z Hz.
